Refinery/Ctx/Split.lean
@@ -6,173 +6,113 @@ variable [HasQuant α]
 
 inductive Var?.Split : Var? α → Var? α → Var? α → Type _
   | neither {A q} : del ⟨A, q⟩ → Split ⟨A, q⟩ ⟨A, 0⟩ ⟨A, 0⟩
-  | left (A q) : Split ⟨A, q⟩ ⟨A, q⟩ ⟨A, 0⟩
-  | right (A q) : Split ⟨A, q⟩ ⟨A, 0⟩ ⟨A, q⟩
-  | both {u} : u.copy → Split u u u
+  | left {v w} (h : v ≤ w) : Split v w v.erase
+  | right {v w} (h : v ≤ w) : Split v v.erase w
+  | sboth {u v w} (hu : u.scopy) (hv : u ≤ v) (hw : u ≤ w) : Split u v w
 
 abbrev Var?.splitN (v : Var? α) [hv : v.del] : v.Split v.erase v.erase := .neither hv
 
-abbrev Var?.splitL (v : Var? α) : v.Split v v.erase := .left v.ty v.q
+abbrev Var?.splitL (v : Var? α) : v.Split v v.erase := .left (le_refl v)
 
-abbrev Var?.splitR (v : Var? α) : v.Split v.erase v := .right v.ty v.q
+abbrev Var?.splitR (v : Var? α) : v.Split v.erase v := .right (le_refl v)
 
-abbrev Var?.splitB (v : Var? α) [hv : v.copy] : v.Split v v := .both hv
+-- abbrev Var?.splitB (v : Var? α) [hv : v.copy] : v.Split v v := .sboth hv (le_refl v) (le_refl v)
 
 theorem Var?.Split.left_unused {u v w : Var? α} (σ : u.Split v w) (h : u.unused) : v.unused
-  := by cases σ <;> first | assumption | rfl
+  := by cases σ <;> (try simp [*]) <;> apply Var?.unused.mono <;> assumption
 
 theorem Var?.Split.right_unused {u v w : Var? α} (σ : u.Split v w) (h : u.unused) : w.unused
-  := by cases σ <;> first | rfl | assumption
+  := by cases σ <;> (try simp [*]) <;> apply Var?.unused.mono <;> assumption
 
 theorem Var?.Split.used_of_left {u v w : Var? α} (σ : u.Split v w) (h : v.used) : u.used
-  := by cases σ <;> first | assumption | cases h
+  := by cases σ
+  <;> first | assumption | cases h | (apply Var?.used.anti (hw := by assumption); assumption)
 
 theorem Var?.Split.used_of_right {u v w : Var? α} (σ : u.Split v w) (h : w.used) : u.used
-  := by cases σ <;> first | cases h | assumption
+  := by cases σ
+  <;> first | assumption | cases h | (apply Var?.used.anti (hw := by assumption); assumption)
 
-theorem Var?.Split.erase_eq_left {u v w : Var? α} (h : u.Split v w)
-  : u.erase = v.erase := by cases h <;> simp [*]
+theorem Var?.Split.erase_eq_left {u v w : Var? α} (σ : u.Split v w)
+  : u.erase = v.erase := by cases σ <;> simp [*]; rename_i h; rw [h.ty]; rename_i h _; rw [h.ty]
 
-theorem Var?.Split.erase_eq_right {u v w : Var? α} (h : u.Split v w)
-  : u.erase = w.erase := by cases h <;> simp [*]
+theorem Var?.Split.erase_eq_right {u v w : Var? α} (σ : u.Split v w)
+  : u.erase = w.erase := by cases σ <;> simp [*]; rename_i h; rw [h.ty]; rename_i _ h; rw [h.ty]
 
-theorem Var?.Split.erase_eq_both {u v w : Var? α} (h : u.Split v w)
-  : v.erase = w.erase := by cases h <;> simp [*]
+theorem Var?.Split.erase_eq_both {u v w : Var? α} (σ : u.Split v w)
+  : v.erase = w.erase := by rw [<-σ.erase_eq_left, <-σ.erase_eq_right]
 
 inductive Ctx?.Split : Ctx? α → Ctx? α → Ctx? α → Type _ where
   | nil : Ctx?.Split .nil .nil .nil
   | cons {Γ Δ Ξ v l r} (h : Split Γ Δ Ξ) (hvw : v.Split l r)
     : Split (Ctx?.cons Γ v) (Ctx?.cons Δ l) (Ctx?.cons Ξ r)
 
+@[simp]
 def Var?.Split.hasLeft {u v w : Var? α} : u.Split v w → Bool
-  | .left _ _ => true | .both _ => true | _ => false
+  | .left _ => true | .sboth _ _ _ => true | _ => false
 
 @[simp]
 theorem Var?.Split.hasLeft_neither {A q} [hA : Var?.del ⟨A, q⟩]
   : (Split.neither (α := α) hA).hasLeft = false := rfl
 
 @[simp]
-theorem Var?.Split.hasLeft_left {A q} : (Split.left (α := α) A q).hasLeft = true := rfl
+theorem Var?.Split.hasLeft_left {v w : Var? α} (h : v ≤ w) : hasLeft (.left h) = true := rfl
 
 @[simp]
-theorem Var?.Split.hasLeft_right {A q} : (Split.right (α := α) A q).hasLeft = false := rfl
+theorem Var?.Split.hasLeft_right {v w : Var? α} (h : v ≤ w) : hasLeft (.right h) = false := rfl
 
 @[simp]
-theorem Var?.Split.hasLeft_both {u : Var? α} [hu : u.copy] : (Split.both hu).hasLeft = true := rfl
+theorem Var?.Split.hasLeft_sboth {u v w : Var? α} (hu : u.scopy) (hv : u ≤ v) (hw : u ≤ w)
+  : hasLeft (.sboth hu hv hw) = true := rfl
 
 def Var?.Split.hasRight {u v w : Var? α} : u.Split v w → Bool
-  | .right _ _ => true | .both _ => true | _ => false
+  | .right _ => true | .sboth _ _ _ => true | _ => false
 
 @[simp]
 theorem Var?.Split.hasRight_neither {A q} [hA : Var?.del ⟨A, q⟩]
   : (Split.neither (α := α) hA).hasRight = false := rfl
 
 @[simp]
-theorem Var?.Split.hasRight_left {A q} : (Split.left (α := α) A q).hasRight = false := rfl
+theorem Var?.Split.hasRight_left {v w : Var? α} (h : v ≤ w) : hasRight (.left h) = false := rfl
 
 @[simp]
-theorem Var?.Split.hasRight_right {A q} : (Split.right (α := α) A q).hasRight = true := rfl
+theorem Var?.Split.hasRight_right {v w : Var? α} (h : v ≤ w) : hasRight (.right h) = true := rfl
 
 @[simp]
-theorem Var?.Split.hasRight_both {u : Var? α} [hu : u.copy] : (Split.both hu).hasRight = true := rfl
+theorem Var?.Split.hasRight_sboth {u v w : Var? α} (hu : u.scopy) (hv : u ≤ v) (hw : u ≤ w)
+  : hasRight (.sboth hu hv hw) = true := rfl
 
-def Var?.Split.wkLeft {u v w : Var? α} (u' : Var? α) (σ : u.Split v w) : Var? α
-  := if u.used && σ.hasLeft then u' else u'.erase
+def Var?.Split.cast {u v w u' v' w' : Var? α}
+  (σ : u.Split v w) (hu : u = u') (hv : v = v') (hw : w = w')
+  : u'.Split v' w'
+  := hu ▸ hv ▸ hw ▸ σ
 
-def Var?.Split.wkRight {u v w : Var? α} (u' : Var? α) (σ : u.Split v w) : Var? α
-  := if u.used && σ.hasRight then u' else u'.erase
+abbrev Var?.Split.cast_src {u v w u': Var? α}
+  (σ : u.Split v w) (hu : u = u')
+  : u'.Split v w
+  := σ.cast hu rfl rfl
 
-@[simp]
-theorem Var?.Split.wkLeft_neither {u' : Var? α} (A q) [hA : Var?.del ⟨A, q⟩]
-  : (Split.neither hA).wkLeft u' = u'.erase := by simp [wkLeft]
+abbrev Var?.Split.cast_left {u v w v' : Var? α}
+  (σ : u.Split v w) (hv : v = v')
+  : u.Split v' w
+  := σ.cast rfl hv rfl
 
-@[simp]
-theorem Var?.Split.wkLeft_left {u' : Var? α} (A q) :
-  (Split.left A q).wkLeft u' = if 1 ≤ q then u' else u'.erase := by simp [wkLeft]
+abbrev Var?.Split.cast_right {u v w w' : Var? α}
+  (σ : u.Split v w) (hw : w = w')
+  : u.Split v w'
+  := σ.cast rfl rfl hw
 
-@[simp]
-theorem Var?.Split.wkLeft_right {u' : Var? α} (A q) :
-  (Split.right A q).wkLeft u' = u'.erase := by simp [wkLeft]
-
-@[simp]
-theorem Var?.Split.wkLeft_both {u' : Var? α} (u : Var? α) [hu : u.copy] :
-  (Split.both hu).wkLeft u' = if u.used then u' else u'.erase := by simp [wkLeft]
-
-@[simp]
-theorem Var?.Split.wkRight_neither {u' : Var? α} (A q) [hA : Var?.del ⟨A, q⟩]
-  : (Split.neither hA).wkRight u' = u'.erase := by simp [wkRight]
-
-@[simp]
-theorem Var?.Split.wkRight_left {u' : Var? α} (A q) :
-  (Split.left A q).wkRight u' = u'.erase := by simp [wkRight]
-
-@[simp]
-theorem Var?.Split.wkRight_right {u' : Var? α} (A q) :
-  (Split.right A q).wkRight u' = if 1 ≤ q then u' else u'.erase := by simp [wkRight]
-
-@[simp]
-theorem Var?.Split.wkRight_both {u' : Var? α} (u : Var? α) [hu : u.copy] :
-  (Split.both hu).wkRight u' = if u.used then u' else u'.erase := by simp [wkRight]
-
-@[simp]
-theorem Var?.Split.wkLeft_unused {u' u v w : Var? α} (σ : u.Split v w) (hu : u.unused) :
-  σ.wkLeft u' = u'.erase := by cases u; cases hu; rfl
-
-@[simp]
-theorem Var?.Split.wkRight_unused {u' u v w : Var? α} (σ : u.Split v w) (hu : u.unused) :
-  σ.wkRight u' = u'.erase := by cases u; cases hu; rfl
-
-@[simp]
-theorem Var?.Split.wkLeft_used {u' u v w : Var? α} (σ : u.Split v w) (hu : u.used) :
-  σ.wkLeft u' = if σ.hasLeft then u' else u'.erase := by rw [wkLeft]; simp [*]
-
-@[simp]
-instance Var?.Split.wkLeft_del {u' u v w : Var? α} [hv : v.del] (ρ : u' ≤ u) (σ : u.Split v w)
-  : (σ.wkLeft u').del := by cases u with | mk A q => cases q using EQuant.casesZero with
-  | zero => simp
-  | rest => cases σ <;> simp [wkLeft] <;> apply Var?.del.anti ρ
-
-@[simp]
-instance Var?.Split.wkLeft_copy {u' u v w : Var? α} [hv : v.copy] (ρ : u' ≤ u) (σ : u.Split v w)
-  : (σ.wkLeft u').copy := by cases u with | mk A q => cases q using EQuant.casesZero with
-  | zero => simp
-  | rest => cases σ <;> simp [wkLeft] <;> apply Var?.copy.anti ρ (by simp)
-
-@[simp]
-instance Var?.Split.wkRight_del {u' u v w : Var? α} [hw : w.del] (ρ : u' ≤ u) (σ : u.Split v w)
-  : (σ.wkRight u').del := by cases u with | mk A q => cases q using EQuant.casesZero with
-  | zero => simp
-  | rest => cases σ <;> simp [wkRight] <;> apply Var?.del.anti ρ
-
-@[simp]
-instance Var?.Split.wkRight_copy {u' u v w : Var? α} [hw : w.copy] (ρ : u' ≤ u) (σ : u.Split v w)
-  : (σ.wkRight u').copy := by cases u with | mk A q => cases q using EQuant.casesZero with
-  | zero => simp
-  | rest => cases σ <;> simp [wkRight] <;> apply Var?.copy.anti ρ (by simp)
-
-def Var?.Split.wk {u' u v w : Var? α} (ρ : u' ≤ u) (σ : u.Split v w) :
-  u'.Split (σ.wkLeft u') (σ.wkRight u') := match u with
-  | ⟨A, 0⟩ => .neither (Var?.del.anti ρ)
-  | ⟨A, (q : Quant)⟩ => match σ with
-    | .neither h => .neither (Var?.del.anti ρ)
-    | .left _ _ => .left _ _
-    | .right _ _ => .right _ _
-    | .both h => .both (Var?.copy.anti ρ (by simp))
-
-theorem Var?.Split.leftWk {u' u v w : Var? α} (ρ : u' ≤ u) (σ : u.Split v w) :
-  σ.wkLeft u' ≤ v := by cases u' with | mk A q' => cases u with | mk _ q =>
-    cases v; cases ρ.ty; cases σ <;> cases q using EQuant.casesZero <;> simp [ρ]
-
-theorem Var?.Split.rightWk {u' u v w : Var? α} (ρ : u' ≤ u) (σ : u.Split v w) :
-  σ.wkRight u' ≤ w := by cases u' with | mk A q' => cases u with | mk _ q =>
-    cases w; cases ρ.ty; cases σ <;> cases q using EQuant.casesZero <;> simp [ρ]
+def Var?.Split.wk {u' u v w : Var? α} (ρ : u' ≤ u) : u.Split v w → u'.Split v w
+  | .neither h => (Split.neither (h.anti ρ)).cast (by simp [ρ.ty]) (by rw [ρ.ty]) (by rw [ρ.ty])
+  | .left h => (Split.left (le_trans ρ h)).cast_right ρ.erase_eq
+  | .right h => (Split.right (le_trans ρ h)).cast_left ρ.erase_eq
+  | .sboth hu hv hw => .sboth (hu.anti ρ) (le_trans ρ hv) (le_trans ρ hw)
 
 @[simp]
 def Var?.Split.comm {u v w : Var? α} : u.Split v w → u.Split w v
   | .neither h => .neither h
-  | .left _ _ => .right _ _
-  | .right _ _ => .left _ _
-  | .both h => .both h
+  | .left h => .right h
+  | .right h => .left h
+  | .sboth hu hv hw => .sboth hu hw hv
 
 @[simp]
 def Ctx?.Split.comm {Γ Δ Ξ : Ctx? α} : Γ.Split Δ Ξ → Γ.Split Ξ Δ
@@ -183,13 +123,13 @@ def Ctx?.Split.comm {Γ Δ Ξ : Ctx? α} : Γ.Split Δ Ξ → Γ.Split Ξ Δ
 def Ctx?.Split.wkLeft {Γ' Γ Δ Ξ : Ctx? α} : Γ'.Wk Γ → Γ.Split Δ Ξ → Ctx? α
   | .nil, _ => .nil
   | .skip (v := v) ρ _, σ => (wkLeft ρ σ).cons v.erase
-  | .cons (v := v) ρ _, .cons σ hlr => (wkLeft ρ σ).cons (hlr.wkLeft v)
+  | .cons (v := v) ρ _, .cons (l := l) σ hlr => (wkLeft ρ σ).cons l
 
 @[simp]
 def Ctx?.Split.wkRight {Γ' Γ Δ Ξ : Ctx? α} : Γ'.Wk Γ → Γ.Split Δ Ξ → Ctx? α
   | .nil, _ => .nil
   | .skip (v := v) ρ _, σ => (wkRight ρ σ).cons v.erase
-  | .cons (v := v) ρ _, .cons σ hlr => (wkRight ρ σ).cons (hlr.wkRight v)
+  | .cons (v := v) ρ _, .cons (r := r) σ hlr => (wkRight ρ σ).cons r
 
 @[simp]
 instance Ctx?.Split.wkLeft_del {Γ' Γ Δ Ξ : Ctx? α} (ρ : Γ'.Wk Γ) (σ : Γ.Split Δ Ξ) [hΔ : Δ.del]
@@ -197,7 +137,7 @@ instance Ctx?.Split.wkLeft_del {Γ' Γ Δ Ξ : Ctx? α} (ρ : Γ'.Wk Γ) (σ : �
   induction ρ generalizing Δ Ξ with
   | cons =>
     cases σ; have _ := hΔ.head; have _ := hΔ.tail;
-    simp [wkLeft, cons_del_iff, Var?.Split.wkLeft_del, *]
+    simp [wkLeft, cons_del_iff, *]
   | _ => simp [*]
 
 @[simp]
@@ -206,7 +146,7 @@ instance Ctx?.Split.wkLeft_copy {Γ' Γ Δ Ξ : Ctx? α} (ρ : Γ'.Wk Γ) (σ : 
   induction ρ generalizing Δ Ξ with
   | cons =>
     cases σ; have _ := hΔ.head; have _ := hΔ.tail;
-    simp [wkLeft, cons_copy_iff, Var?.Split.wkLeft_copy, *]
+    simp [wkLeft, cons_copy_iff, *]
   | _ => simp [*]
 
 @[simp]
@@ -215,7 +155,7 @@ instance Ctx?.Split.wkRight_del {Γ' Γ Δ Ξ : Ctx? α} (ρ : Γ'.Wk Γ) (σ : 
   induction ρ generalizing Δ Ξ with
   | cons =>
     cases σ; have _ := hΞ.head; have _ := hΞ.tail;
-    simp [wkRight, cons_del_iff, Var?.Split.wkRight_del, *]
+    simp [wkRight, cons_del_iff, *]
   | _ => simp [*]
 
 @[simp]
@@ -224,7 +164,7 @@ instance Ctx?.Split.wkRight_copy {Γ' Γ Δ Ξ : Ctx? α} (ρ : Γ'.Wk Γ) (σ :
   induction ρ generalizing Δ Ξ with
   | cons =>
     cases σ; have _ := hΞ.head; have _ := hΞ.tail;
-    simp [wkRight, cons_copy_iff, Var?.Split.wkRight_copy, *]
+    simp [wkRight, cons_copy_iff, *]
   | _ => simp [*]
 
 def Ctx?.Split.wk {Γ' Γ Δ Ξ : Ctx? α}
@@ -237,13 +177,13 @@ def Ctx?.Split.wk {Γ' Γ Δ Ξ : Ctx? α}
 def Ctx?.Split.leftWk {Γ' Γ Δ Ξ : Ctx? α} : (ρ : Γ'.Wk Γ) → (σ : Γ.Split Δ Ξ) → (σ.wkLeft ρ).Wk Δ
   | .nil, .nil => .nil
   | .skip ρ _, σ => .skip (σ.leftWk ρ) inferInstance
-  | .cons (v := v) ρ hvw, .cons σ hlr => .cons (σ.leftWk ρ) (hlr.leftWk hvw)
+  | .cons (v := v) ρ _, .cons σ hlr => .cons (σ.leftWk ρ) (le_refl _)
 
 @[simp]
 def Ctx?.Split.rightWk {Γ' Γ Δ Ξ : Ctx? α} : (ρ : Γ'.Wk Γ) → (σ : Γ.Split Δ Ξ) → (σ.wkRight ρ).Wk Ξ
   | .nil, .nil => .nil
   | .skip ρ _, σ => .skip (σ.rightWk ρ) inferInstance
-  | .cons (v := v) ρ hvw, .cons σ hlr => .cons (σ.rightWk ρ) (hlr.rightWk hvw)
+  | .cons (v := v) ρ _, .cons σ hlr => .cons (σ.rightWk ρ) (le_refl _)
 
 @[simp]
 theorem Ctx?.Split.ix_leftWk {Γ' Γ Δ Ξ : Ctx? α} (ρ : Γ'.Wk Γ) (σ : Γ.Split Δ Ξ)
@@ -263,286 +203,286 @@ theorem Ctx?.Split.rightWk_applied {Γ' Γ Δ Ξ : Ctx? α} (ρ : Γ'.Wk Γ) (σ
 
 @[simp]
 def Var?.Split.leftCtx {u v w : Var? α} : u.Split v w → Ctx? α → Ctx? α
-  | .left _ _, Γ | .both _, Γ => Γ
-  | .right _ _, Γ | .neither _, Γ => Γ.erase
+  | .left _, Γ | .sboth _ _ _, Γ => Γ
+  | .right _, Γ | .neither _, Γ => Γ.erase
 
 @[simp]
 def Var?.Split.rightCtx {u v w : Var? α} : u.Split v w → Ctx? α → Ctx? α
-  | .left _ _, Γ | .neither _, Γ => Γ.erase
-  | .right _ _, Γ | .both _, Γ => Γ
+  | .left _, Γ | .neither _, Γ => Γ.erase
+  | .right _, Γ | .sboth _ _ _, Γ => Γ
 
-def Var?.Split.v12_3_23 {u₁₂₃ u₁₂ u₁ u₂ u₃ : Var? α} : u₁₂₃.Split u₁₂ u₃ → u₁₂.Split u₁ u₂ → Var? α
-  | .neither _, _ | .left _ _, .neither _ | .left _ _, .left _ _ => u₁₂₃.erase
-  | _, _ => u₁₂₃
+-- def Var?.Split.v12_3_23 {u₁₂₃ u₁₂ u₁ u₂ u₃ : Var? α} : u₁₂₃.Split u₁₂ u₃ → u₁₂.Split u₁ u₂ → Var? α
+--   | .neither _, _ | .left _, .neither _ | .left _, .left _ => u₁₂₃.erase
+--   | _, _ => u₁₂₃
 
-@[simp]
-instance Var?.Split.v12_3_23_del {u₁₂₃ u₁₂ u₁ u₂ u₃ : Var? α}
-  (h12_3 : u₁₂₃.Split u₁₂ u₃) (h12 : u₁₂.Split u₁ u₂) [h2 : u₂.del] [h3 : u₃.del]
-  : (h12_3.v12_3_23 h12).del
-  := by cases h12_3 <;> cases h12 <;> assumption
+-- @[simp]
+-- instance Var?.Split.v12_3_23_del {u₁₂₃ u₁₂ u₁ u₂ u₃ : Var? α}
+--   (h12_3 : u₁₂₃.Split u₁₂ u₃) (h12 : u₁₂.Split u₁ u₂) [h2 : u₂.del] [h3 : u₃.del]
+--   : (h12_3.v12_3_23 h12).del
+--   := by cases h12_3 <;> cases h12 <;> simp [v12_3_23]
 
-@[simp]
-instance Var?.Split.v12_3_23_copy {u₁₂₃ u₁₂ u₁ u₂ u₃ : Var? α}
-  (h12_3 : u₁₂₃.Split u₁₂ u₃) (h12 : u₁₂.Split u₁ u₂) [h2 : u₂.copy] [h3 : u₃.copy]
-  : (h12_3.v12_3_23 h12).copy
-  := by cases h12_3 <;> cases h12 <;> simp [v12_3_23, *]
+-- @[simp]
+-- instance Var?.Split.v12_3_23_copy {u₁₂₃ u₁₂ u₁ u₂ u₃ : Var? α}
+--   (h12_3 : u₁₂₃.Split u₁₂ u₃) (h12 : u₁₂.Split u₁ u₂) [h2 : u₂.copy] [h3 : u₃.copy]
+--   : (h12_3.v12_3_23 h12).copy
+--   := by cases h12_3 <;> cases h12 <;> sorry
 
-def Var?.Split.s12_3_1_23 {u₁₂₃ u₁₂ u₁ u₂ u₃ : Var? α}
-  : (h12_3 : u₁₂₃.Split u₁₂ u₃) → (h12 : u₁₂.Split u₁ u₂) → u₁₂₃.Split u₁ (h12_3.v12_3_23 h12)
-  | .neither h, .neither _
-  | .neither h, .left _ _
-  | .neither h, .right _ _
-  | .neither h, .both _
-  | .left _ _, .neither h => .neither h
-  | .left _ _, .left _ _ => .left _ _
-  | .left _ _, .right _ _ => .right _ _
-  | .left _ _, .both h => .both h
-  | .right _ _, .neither _
-  | .right _ _, .left _ _
-  | .right _ _, .right _ _
-  | .right _ _, .both h => .right _ _
-  | .both h, .neither _ => .right _ _
-  | .both h, .left _ _ => .both h
-  | .both _, .right _ _ => .right _ _
-  | .both h, .both _ => .both h
+-- def Var?.Split.s12_3_1_23 {u₁₂₃ u₁₂ u₁ u₂ u₃ : Var? α}
+--   : (h12_3 : u₁₂₃.Split u₁₂ u₃) → (h12 : u₁₂.Split u₁ u₂) → u₁₂₃.Split u₁ (h12_3.v12_3_23 h12)
+--   | .neither h, .neither _ => sorry -- neither
+--   | .neither h, .left hvw => sorry -- neither
+--   | .neither h, .right _ => sorry -- neither
+--   | .neither h, .sboth _ _ _ => sorry -- neither
+--   | .left _, .neither h => sorry -- neither
+--   | .left _, .left _ => sorry -- left
+--   | .left _, .right _ => sorry -- right
+--   | .left _, .sboth h _ _ => sorry -- both
+--   | .right _, .neither _ => sorry -- right
+--   | .right _, .left _ => sorry -- right
+--   | .right _, .right _ => sorry -- right
+--   | .right _, .sboth h _ _ => sorry -- right
+--   | .sboth h _ _, .neither _ => sorry -- right
+--   | .sboth h _ _, .left _ => sorry -- both
+--   | .sboth _ _ _, .right _ => sorry -- right
+--   | .sboth h _ _, .sboth _ _ _ => sorry -- both
 
-def Var?.Split.s12_3_23 {u₁₂₃ u₁₂ u₁ u₂ u₃ : Var? α}
-  : (h12_3 : u₁₂₃.Split u₁₂ u₃) → (h12 : u₁₂.Split u₁ u₂) → (h12_3.v12_3_23 h12).Split u₂ u₃
-  | .neither _, .neither _
-  | .neither _, .left _ _
-  | .neither _, .right _ _
-  | .neither _, .both _
-  | .left _ _, .neither h => .neither inferInstance
-  | .left _ _, .left _ _ => .left _ _
-  | .left _ _, .right _ _ => .left _ _
-  | .left _ _, .both h => .left _ _
-  | .right _ _, .neither _
-  | .right _ _, .left _ _
-  | .right _ _, .right _ _
-  | .right _ _, .both h => .right _ _
-  | .both _, .neither _ => .right _ _
-  | .both _, .left _ _ => .right _ _
-  | .both h, .right _ _ => .both h
-  | .both h, .both _ => .both h
+-- def Var?.Split.s12_3_23 {u₁₂₃ u₁₂ u₁ u₂ u₃ : Var? α}
+--   : (h12_3 : u₁₂₃.Split u₁₂ u₃) → (h12 : u₁₂.Split u₁ u₂) → (h12_3.v12_3_23 h12).Split u₂ u₃
+--   | .neither _, .neither _ => sorry -- neither
+--   | .neither _, .left _ => sorry -- neither
+--   | .neither _, .right _ => sorry -- neither
+--   | .neither _, .sboth _ _ _ => sorry -- neither
+--   | .left _, .neither _ => sorry -- neither
+--   | .left _, .left _ => sorry -- left
+--   | .left _, .right _ => sorry -- left
+--   | .left _, .sboth h _ _ => sorry -- left
+--   | .right _, .neither _ => sorry -- right
+--   | .right _, .left _ => sorry -- right
+--   | .right _, .right _ => sorry -- right
+--   | .right _, .sboth h _ _ => sorry -- right
+--   | .sboth _ _ _, .neither _ => sorry -- right
+--   | .sboth _ _ _, .left _ => sorry -- right
+--   | .sboth h _ _, .right _ => sorry -- both
+--   | .sboth h _ _, .sboth _ _ _ => sorry -- both
 
-def Var?.Split.v1_23_12 {u₁₂₃ u₂₃ u₁ u₂ u₃ : Var? α}
-  : u₁₂₃.Split u₁ u₂₃ → u₂₃.Split u₂ u₃ → Var? α
-  | .neither _, _ | .right _ _, .neither _ | .right _ _, .right _ _ => u₁₂₃.erase
-  | _, _ => u₁₂₃
+-- def Var?.Split.v1_23_12 {u₁₂₃ u₂₃ u₁ u₂ u₃ : Var? α}
+--   : u₁₂₃.Split u₁ u₂₃ → u₂₃.Split u₂ u₃ → Var? α
+--   | .neither _, _ | .right _, .neither _ | .right _, .right _ => u₁₂₃.erase
+--   | _, _ => u₁₂₃
 
-@[simp]
-instance Var?.Split.v1_23_12_del {u₁₂₃ u₂₃ u₁ u₂ u₃ : Var? α}
-  (h1_23 : u₁₂₃.Split u₁ u₂₃) (h23 : u₂₃.Split u₂ u₃) [h1 : u₁.del] [h2 : u₂.del]
-  : (h1_23.v1_23_12 h23).del
-  := by cases h1_23 <;> cases h23 <;> assumption
+-- @[simp]
+-- instance Var?.Split.v1_23_12_del {u₁₂₃ u₂₃ u₁ u₂ u₃ : Var? α}
+--   (h1_23 : u₁₂₃.Split u₁ u₂₃) (h23 : u₂₃.Split u₂ u₃) [h1 : u₁.del] [h2 : u₂.del]
+--   : (h1_23.v1_23_12 h23).del
+--   := by cases h1_23 <;> cases h23 <;> sorry
 
-@[simp]
-instance Var?.Split.v1_23_12_copy {u₁₂₃ u₂₃ u₁ u₂ u₃ : Var? α}
-  (h1_23 : u₁₂₃.Split u₁ u₂₃) (h23 : u₂₃.Split u₂ u₃) [h1 : u₁.copy] [h2 : u₂.copy]
-  : (h1_23.v1_23_12 h23).copy
-  := by cases h1_23 <;> cases h23 <;> simp [v1_23_12, *]
+-- @[simp]
+-- instance Var?.Split.v1_23_12_copy {u₁₂₃ u₂₃ u₁ u₂ u₃ : Var? α}
+--   (h1_23 : u₁₂₃.Split u₁ u₂₃) (h23 : u₂₃.Split u₂ u₃) [h1 : u₁.copy] [h2 : u₂.copy]
+--   : (h1_23.v1_23_12 h23).copy
+--   := by cases h1_23 <;> cases h23 <;> sorry
 
-def Var?.Split.s1_23_12_3 {u₁₂₃ u₂₃ u₁ u₂ u₃ : Var? α}
-  : (h1 : u₁₂₃.Split u₁ u₂₃) → (h23 : u₂₃.Split u₂ u₃) → u₁₂₃.Split (h1.v1_23_12 h23) u₃
-  | .neither h, .neither _
-  | .neither h, .left _ _
-  | .neither h, .right _ _
-  | .neither h, .both _
-  | .right _ _, .neither h => .neither h
-  | .left _ _ , .neither _
-  | .left _ _, .left _ _
-  | .left _ _, .right _ _
-  | .left _ _, .both _ => .left _ _
-  | .right _ _, .left _ _ => .left _ _
-  | .right _ _, .right _ _ => .right _ _
-  | .right _ _, .both h => .both h
-  | .both _, .neither h => .left _ _
-  | .both h, .left _ _ => .left _ _
-  | .both h, .right _ _ => .both h
-  | .both h, .both _ => .both h
+-- def Var?.Split.s1_23_12_3 {u₁₂₃ u₂₃ u₁ u₂ u₃ : Var? α}
+--   : (h1 : u₁₂₃.Split u₁ u₂₃) → (h23 : u₂₃.Split u₂ u₃) → u₁₂₃.Split (h1.v1_23_12 h23) u₃
+--   | .neither h, .neither _ => sorry -- neither
+--   | .neither h, .left _ => sorry -- neither
+--   | .neither h, .right _ => sorry -- neither
+--   | .neither h, .sboth _ _ _ => sorry -- neither
+--   | .right _, .neither h => sorry -- neither
+--   | .left _ , .neither _ => sorry -- left
+--   | .left _, .left _ => sorry -- left
+--   | .left _, .right _ => sorry -- left
+--   | .left _, .sboth _ _ _ => sorry -- left
+--   | .right _, .left _ => sorry -- left
+--   | .right _, .right _ => sorry -- right
+--   | .right _, .sboth h _ _ => sorry -- both
+--   | .sboth _ _ _, .neither h => sorry -- left
+--   | .sboth h _ _, .left _ => sorry -- left
+--   | .sboth h _ _, .right _ => sorry -- both
+--   | .sboth h _ _, .sboth _ _ _ => sorry -- both
 
-def Var?.Split.s1_23_12 {u₁₂₃ u₂₃ u₁ u₂ u₃ : Var? α}
-  : (h1 : u₁₂₃.Split u₁ u₂₃) → (h23 : u₂₃.Split u₂ u₃) → (h1.v1_23_12 h23).Split u₁ u₂
-  | .neither _, .neither _
-  | .neither _, .left _ _
-  | .neither _, .right _ _
-  | .neither _, .both _
-  | .right _ _, .neither _ => .neither inferInstance
-  | .left _ _, .neither _ => .left _ _
-  | .left _ _, .left _ _ => .left _ _
-  | .left _ _, .right _ _ => .left _ _
-  | .left _ _, .both _ => .left _ _
-  | .right _ _, .left _ _ => .right _ _
-  | .right _ _, .right _ _ => .right _ _
-  | .right _ _, .both _ => .right _ _
-  | .both _, .neither _ => .left _ _
-  | .both h, .left _ _ => .both h
-  | .both _, .right _ _ => .left _ _
-  | .both h, .both _ => .both h
+-- def Var?.Split.s1_23_12 {u₁₂₃ u₂₃ u₁ u₂ u₃ : Var? α}
+--   : (h1 : u₁₂₃.Split u₁ u₂₃) → (h23 : u₂₃.Split u₂ u₃) → (h1.v1_23_12 h23).Split u₁ u₂
+--   | .neither _, .neither _ => sorry -- neither
+--   | .neither _, .left _  => sorry -- neither
+--   | .neither _, .right _ => sorry -- neither
+--   | .neither _, .sboth _ _ _ => sorry -- neither
+--   | .right _, .neither _ => sorry -- neither
+--   | .left _, .neither _ => sorry -- left
+--   | .left _, .left _ => sorry -- left
+--   | .left _, .right _ => sorry -- left
+--   | .left _, .sboth _ _ _ => sorry -- left
+--   | .right _, .left _ => sorry -- right
+--   | .right _, .right _ => sorry -- right
+--   | .right _, .sboth _ _ _ => sorry -- right
+--   | .sboth _ _ _, .neither _ => sorry -- left
+--   | .sboth h _ _, .left _ => sorry -- both
+--   | .sboth _ _ _, .right _ => sorry -- left
+--   | .sboth h _ _, .sboth _ _ _ => sorry -- both
 
-def Ctx?.Split.c1_23_12 {Γ₁₂₃ Γ₂₃ Γ₁ Γ₂ Γ₃ : Ctx? α}
-  : Γ₁₂₃.Split Γ₁ Γ₂₃ → Γ₂₃.Split Γ₂ Γ₃ → Ctx? α
-  | .nil, .nil => .nil
-  | .cons h hvw, .cons h' hvw' => .cons (h.c1_23_12 h') (hvw.v1_23_12 hvw')
+-- def Ctx?.Split.c1_23_12 {Γ₁₂₃ Γ₂₃ Γ₁ Γ₂ Γ₃ : Ctx? α}
+--   : Γ₁₂₃.Split Γ₁ Γ₂₃ → Γ₂₃.Split Γ₂ Γ₃ → Ctx? α
+--   | .nil, .nil => .nil
+--   | .cons h hvw, .cons h' hvw' => .cons (h.c1_23_12 h') (hvw.v1_23_12 hvw')
 
-@[simp]
-instance Ctx?.Split.c1_23_12_del {Γ₁₂₃ Γ₂₃ Γ₁ Γ₂ Γ₃ : Ctx? α}
-  (h12_3 : Γ₁₂₃.Split Γ₁ Γ₂₃) (h23 : Γ₂₃.Split Γ₂ Γ₃) [h1 : Γ₁.del] [h2 : Γ₂.del]
-  : (h12_3.c1_23_12 h23).del
-  := by
-  generalize h1 = h1
-  induction h12_3 generalizing Γ₂ Γ₃ <;> cases h23
-  simp [c1_23_12]
-  simp [c1_23_12, h2.head, h2.tail, h1.head, h1.tail, *]
+-- @[simp]
+-- instance Ctx?.Split.c1_23_12_del {Γ₁₂₃ Γ₂₃ Γ₁ Γ₂ Γ₃ : Ctx? α}
+--   (h12_3 : Γ₁₂₃.Split Γ₁ Γ₂₃) (h23 : Γ₂₃.Split Γ₂ Γ₃) [h1 : Γ₁.del] [h2 : Γ₂.del]
+--   : (h12_3.c1_23_12 h23).del
+--   := by
+--   generalize h1 = h1
+--   induction h12_3 generalizing Γ₂ Γ₃ <;> cases h23
+--   simp [c1_23_12]
+--   simp [c1_23_12, h2.head, h2.tail, h1.head, h1.tail, *]
 
-@[simp]
-instance Ctx?.Split.c1_23_12_copy {Γ₁₂₃ Γ₂₃ Γ₁ Γ₂ Γ₃ : Ctx? α}
-  (h12_3 : Γ₁₂₃.Split Γ₁ Γ₂₃) (h23 : Γ₂₃.Split Γ₂ Γ₃) [h1 : Γ₁.copy] [h2 : Γ₂.copy]
-  : (h12_3.c1_23_12 h23).copy
-  := by
-  generalize h1 = h1
-  induction h12_3 generalizing Γ₂ Γ₃ <;> cases h23
-  simp [c1_23_12]
-  simp [c1_23_12, h2.head, h2.tail, h1.head, h1.tail, *]
+-- @[simp]
+-- instance Ctx?.Split.c1_23_12_copy {Γ₁₂₃ Γ₂₃ Γ₁ Γ₂ Γ₃ : Ctx? α}
+--   (h12_3 : Γ₁₂₃.Split Γ₁ Γ₂₃) (h23 : Γ₂₃.Split Γ₂ Γ₃) [h1 : Γ₁.copy] [h2 : Γ₂.copy]
+--   : (h12_3.c1_23_12 h23).copy
+--   := by
+--   generalize h1 = h1
+--   induction h12_3 generalizing Γ₂ Γ₃ <;> cases h23
+--   simp [c1_23_12]
+--   simp [c1_23_12, h2.head, h2.tail, h1.head, h1.tail, *]
 
-def Ctx?.Split.s1_23_12_3 {Γ₁₂₃ Γ₂₃ Γ₁ Γ₂ Γ₃ : Ctx? α}
-  : (h12_3 : Γ₁₂₃.Split Γ₁ Γ₂₃) → (h23 : Γ₂₃.Split Γ₂ Γ₃)
-    → Γ₁₂₃.Split (h12_3.c1_23_12 h23) Γ₃
-  | .nil, .nil => .nil
-  | .cons h hvw, .cons h' hvw' => .cons (s1_23_12_3 h h') (Var?.Split.s1_23_12_3 hvw hvw')
+-- def Ctx?.Split.s1_23_12_3 {Γ₁₂₃ Γ₂₃ Γ₁ Γ₂ Γ₃ : Ctx? α}
+--   : (h12_3 : Γ₁₂₃.Split Γ₁ Γ₂₃) → (h23 : Γ₂₃.Split Γ₂ Γ₃)
+--     → Γ₁₂₃.Split (h12_3.c1_23_12 h23) Γ₃
+--   | .nil, .nil => .nil
+--   | .cons h hvw, .cons h' hvw' => .cons (s1_23_12_3 h h') (Var?.Split.s1_23_12_3 hvw hvw')
 
-def Ctx?.Split.s1_23_12 {Γ₁₂₃ Γ₂₃ Γ₁ Γ₂ Γ₃ : Ctx? α}
-  : (h12_3 : Γ₁₂₃.Split Γ₁ Γ₂₃) → (h23 : Γ₂₃.Split Γ₂ Γ₃) → (h12_3.c1_23_12 h23).Split Γ₁ Γ₂
-  | .nil, .nil => .nil
-  | .cons h hvw, .cons h' hvw' => .cons (s1_23_12 h h') (Var?.Split.s1_23_12 hvw hvw')
+-- def Ctx?.Split.s1_23_12 {Γ₁₂₃ Γ₂₃ Γ₁ Γ₂ Γ₃ : Ctx? α}
+--   : (h12_3 : Γ₁₂₃.Split Γ₁ Γ₂₃) → (h23 : Γ₂₃.Split Γ₂ Γ₃) → (h12_3.c1_23_12 h23).Split Γ₁ Γ₂
+--   | .nil, .nil => .nil
+--   | .cons h hvw, .cons h' hvw' => .cons (s1_23_12 h h') (Var?.Split.s1_23_12 hvw hvw')
 
-def Ctx?.Split.c12_3_23 {Γ₁₂₃ Γ₁₂ Γ₁ Γ₂ Γ₃ : Ctx? α}
-  : Γ₁₂₃.Split Γ₁₂ Γ₃ → Γ₁₂.Split Γ₁ Γ₂ → Ctx? α
-  | .nil, .nil => .nil
-  | .cons h hvw, .cons h' hvw' => .cons (c12_3_23 h h') (Var?.Split.v12_3_23 hvw hvw')
+-- def Ctx?.Split.c12_3_23 {Γ₁₂₃ Γ₁₂ Γ₁ Γ₂ Γ₃ : Ctx? α}
+--   : Γ₁₂₃.Split Γ₁₂ Γ₃ → Γ₁₂.Split Γ₁ Γ₂ → Ctx? α
+--   | .nil, .nil => .nil
+--   | .cons h hvw, .cons h' hvw' => .cons (c12_3_23 h h') (Var?.Split.v12_3_23 hvw hvw')
 
-@[simp]
-instance Ctx?.Split.c12_3_23_del {Γ₁₂₃ Γ₁₂ Γ₁ Γ₂ Γ₃ : Ctx? α}
-  (h12_3 : Γ₁₂₃.Split Γ₁₂ Γ₃) (h12 : Γ₁₂.Split Γ₁ Γ₂) [h2 : Γ₂.del] [h3 : Γ₃.del]
-  : (h12_3.c12_3_23 h12).del
-  := by
-  generalize h3 = h3
-  induction h12_3 generalizing Γ₁ Γ₂ <;> cases h12
-  simp [c12_3_23]
-  simp [c12_3_23, h2.head, h2.tail, h3.head, h3.tail, *]
+-- @[simp]
+-- instance Ctx?.Split.c12_3_23_del {Γ₁₂₃ Γ₁₂ Γ₁ Γ₂ Γ₃ : Ctx? α}
+--   (h12_3 : Γ₁₂₃.Split Γ₁₂ Γ₃) (h12 : Γ₁₂.Split Γ₁ Γ₂) [h2 : Γ₂.del] [h3 : Γ₃.del]
+--   : (h12_3.c12_3_23 h12).del
+--   := by
+--   generalize h3 = h3
+--   induction h12_3 generalizing Γ₁ Γ₂ <;> cases h12
+--   simp [c12_3_23]
+--   simp [c12_3_23, h2.head, h2.tail, h3.head, h3.tail, *]
 
-@[simp]
-instance Ctx?.Split.c12_3_23_copy {Γ₁₂₃ Γ₁₂ Γ₁ Γ₂ Γ₃ : Ctx? α}
-  (h12_3 : Γ₁₂₃.Split Γ₁₂ Γ₃) (h12 : Γ₁₂.Split Γ₁ Γ₂) [h2 : Γ₂.copy] [h3 : Γ₃.copy]
-  : (h12_3.c12_3_23 h12).copy
-  := by
-  generalize h3 = h3
-  induction h12_3 generalizing Γ₁ Γ₂ <;> cases h12
-  simp [c12_3_23]
-  simp [c12_3_23, h2.head, h2.tail, h3.head, h3.tail, *]
+-- @[simp]
+-- instance Ctx?.Split.c12_3_23_copy {Γ₁₂₃ Γ₁₂ Γ₁ Γ₂ Γ₃ : Ctx? α}
+--   (h12_3 : Γ₁₂₃.Split Γ₁₂ Γ₃) (h12 : Γ₁₂.Split Γ₁ Γ₂) [h2 : Γ₂.copy] [h3 : Γ₃.copy]
+--   : (h12_3.c12_3_23 h12).copy
+--   := by
+--   generalize h3 = h3
+--   induction h12_3 generalizing Γ₁ Γ₂ <;> cases h12
+--   simp [c12_3_23]
+--   simp [c12_3_23, h2.head, h2.tail, h3.head, h3.tail, *]
 
-def Ctx?.Split.s12_3_1_23 {Γ₁₂₃ Γ₁₂ Γ₁ Γ₂ Γ₃ : Ctx? α}
-  : (h12_3 : Γ₁₂₃.Split Γ₁₂ Γ₃) → (h12 : Γ₁₂.Split Γ₁ Γ₂)
-    → Γ₁₂₃.Split Γ₁ (h12_3.c12_3_23 h12)
-  | .nil, .nil => .nil
-  | .cons h hvw, .cons h' hvw' => .cons (s12_3_1_23 h h') (Var?.Split.s12_3_1_23 hvw hvw')
+-- def Ctx?.Split.s12_3_1_23 {Γ₁₂₃ Γ₁₂ Γ₁ Γ₂ Γ₃ : Ctx? α}
+--   : (h12_3 : Γ₁₂₃.Split Γ₁₂ Γ₃) → (h12 : Γ₁₂.Split Γ₁ Γ₂)
+--     → Γ₁₂₃.Split Γ₁ (h12_3.c12_3_23 h12)
+--   | .nil, .nil => .nil
+--   | .cons h hvw, .cons h' hvw' => .cons (s12_3_1_23 h h') (Var?.Split.s12_3_1_23 hvw hvw')
 
-def Ctx?.Split.s12_3_23 {Γ₁₂₃ Γ₁₂ Γ₁ Γ₂ Γ₃ : Ctx? α}
-  : (h12_3 : Γ₁₂₃.Split Γ₁₂ Γ₃) → (h12 : Γ₁₂.Split Γ₁ Γ₂) → (h12_3.c12_3_23 h12).Split Γ₂ Γ₃
-  | .nil, .nil => .nil
-  | .cons h hvw, .cons h' hvw' => .cons (s12_3_23 h h') (Var?.Split.s12_3_23 hvw hvw')
+-- def Ctx?.Split.s12_3_23 {Γ₁₂₃ Γ₁₂ Γ₁ Γ₂ Γ₃ : Ctx? α}
+--   : (h12_3 : Γ₁₂₃.Split Γ₁₂ Γ₃) → (h12 : Γ₁₂.Split Γ₁ Γ₂) → (h12_3.c12_3_23 h12).Split Γ₂ Γ₃
+--   | .nil, .nil => .nil
+--   | .cons h hvw, .cons h' hvw' => .cons (s12_3_23 h h') (Var?.Split.s12_3_23 hvw hvw')
 
-abbrev Ctx?.Split.c12_3_13 {Γ₁₂₃ Γ₁₂ Γ₁ Γ₂ Γ₃ : Ctx? α}
-  (h12_3 : Γ₁₂₃.Split Γ₁₂ Γ₃) (h12 : Γ₁₂.Split Γ₁ Γ₂)
-  : Ctx? α := h12_3.comm.c1_23_12 h12
+-- abbrev Ctx?.Split.c12_3_13 {Γ₁₂₃ Γ₁₂ Γ₁ Γ₂ Γ₃ : Ctx? α}
+--   (h12_3 : Γ₁₂₃.Split Γ₁₂ Γ₃) (h12 : Γ₁₂.Split Γ₁ Γ₂)
+--   : Ctx? α := h12_3.comm.c1_23_12 h12
 
-theorem Ctx?.Split.c12_3_13_del {Γ₁₂₃ Γ₁₂ Γ₁ Γ₂ Γ₃ : Ctx? α}
-  (h12_3 : Γ₁₂₃.Split Γ₁₂ Γ₃) (h12 : Γ₁₂.Split Γ₁ Γ₂) [h1 : Γ₁.del] [h3 : Γ₃.del]
-  : (h12_3.c12_3_13 h12).del := inferInstance
+-- theorem Ctx?.Split.c12_3_13_del {Γ₁₂₃ Γ₁₂ Γ₁ Γ₂ Γ₃ : Ctx? α}
+--   (h12_3 : Γ₁₂₃.Split Γ₁₂ Γ₃) (h12 : Γ₁₂.Split Γ₁ Γ₂) [h1 : Γ₁.del] [h3 : Γ₃.del]
+--   : (h12_3.c12_3_13 h12).del := inferInstance
 
-theorem Ctx?.Split.c12_3_13_copy {Γ₁₂₃ Γ₁₂ Γ₁ Γ₂ Γ₃ : Ctx? α}
-  (h12_3 : Γ₁₂₃.Split Γ₁₂ Γ₃) (h12 : Γ₁₂.Split Γ₁ Γ₂) [h1 : Γ₁.copy] [h3 : Γ₃.copy]
-  : (h12_3.c12_3_13 h12).copy := inferInstance
+-- theorem Ctx?.Split.c12_3_13_copy {Γ₁₂₃ Γ₁₂ Γ₁ Γ₂ Γ₃ : Ctx? α}
+--   (h12_3 : Γ₁₂₃.Split Γ₁₂ Γ₃) (h12 : Γ₁₂.Split Γ₁ Γ₂) [h1 : Γ₁.copy] [h3 : Γ₃.copy]
+--   : (h12_3.c12_3_13 h12).copy := inferInstance
 
-abbrev Ctx?.Split.s12_3_13_2 {Γ₁₂₃ Γ₁₂ Γ₁ Γ₂ Γ₃ : Ctx? α}
-  (h12_3 : Γ₁₂₃.Split Γ₁₂ Γ₃) (h12 : Γ₁₂.Split Γ₁ Γ₂)
-  : Γ₁₂₃.Split (h12_3.c12_3_13 h12) Γ₂
-  := h12_3.comm.s1_23_12_3 h12
+-- abbrev Ctx?.Split.s12_3_13_2 {Γ₁₂₃ Γ₁₂ Γ₁ Γ₂ Γ₃ : Ctx? α}
+--   (h12_3 : Γ₁₂₃.Split Γ₁₂ Γ₃) (h12 : Γ₁₂.Split Γ₁ Γ₂)
+--   : Γ₁₂₃.Split (h12_3.c12_3_13 h12) Γ₂
+--   := h12_3.comm.s1_23_12_3 h12
 
-abbrev Ctx?.Split.s12_3_31 {Γ₁₂₃ Γ₁₂ Γ₁ Γ₂ Γ₃ : Ctx? α}
-  (h12_3 : Γ₁₂₃.Split Γ₁₂ Γ₃) (h12 : Γ₁₂.Split Γ₁ Γ₂)
-  : (h12_3.c12_3_13 h12).Split Γ₃ Γ₁
-  := h12_3.comm.s1_23_12 h12
+-- abbrev Ctx?.Split.s12_3_31 {Γ₁₂₃ Γ₁₂ Γ₁ Γ₂ Γ₃ : Ctx? α}
+--   (h12_3 : Γ₁₂₃.Split Γ₁₂ Γ₃) (h12 : Γ₁₂.Split Γ₁ Γ₂)
+--   : (h12_3.c12_3_13 h12).Split Γ₃ Γ₁
+--   := h12_3.comm.s1_23_12 h12
 
-abbrev Ctx?.Split.s12_3_13 {Γ₁₂₃ Γ₁₂ Γ₁ Γ₂ Γ₃ : Ctx? α}
-  (h12_3 : Γ₁₂₃.Split Γ₁₂ Γ₃) (h12 : Γ₁₂.Split Γ₁ Γ₂)
-  : (h12_3.c12_3_13 h12).Split Γ₁ Γ₃
-  := (h12_3.s12_3_31 h12).comm
+-- abbrev Ctx?.Split.s12_3_13 {Γ₁₂₃ Γ₁₂ Γ₁ Γ₂ Γ₃ : Ctx? α}
+--   (h12_3 : Γ₁₂₃.Split Γ₁₂ Γ₃) (h12 : Γ₁₂.Split Γ₁ Γ₂)
+--   : (h12_3.c12_3_13 h12).Split Γ₁ Γ₃
+--   := (h12_3.s12_3_31 h12).comm
 
-abbrev Ctx?.Split.c12_34_123 {Γ₁₂₃₄ Γ₁₂ Γ₃₄ Γ₃ Γ₄ : Ctx? α}
-  (h12_34 : Γ₁₂₃₄.Split Γ₁₂ Γ₃₄) (h34 : Γ₃₄.Split Γ₃ Γ₄)
-  : Ctx? α := h12_34.c1_23_12 h34
+-- abbrev Ctx?.Split.c12_34_123 {Γ₁₂₃₄ Γ₁₂ Γ₃₄ Γ₃ Γ₄ : Ctx? α}
+--   (h12_34 : Γ₁₂₃₄.Split Γ₁₂ Γ₃₄) (h34 : Γ₃₄.Split Γ₃ Γ₄)
+--   : Ctx? α := h12_34.c1_23_12 h34
 
-theorem Ctx?.Split.c12_34_123_del {Γ₁₂₃₄ Γ₁₂ Γ₃₄ Γ₃ Γ₄ : Ctx? α}
-  (h12_34 : Γ₁₂₃₄.Split Γ₁₂ Γ₃₄) (h34 : Γ₃₄.Split Γ₃ Γ₄) [h12 : Γ₁₂.del] [h3 : Γ₃.del]
-  : (h12_34.c12_34_123 h34).del := inferInstance
+-- theorem Ctx?.Split.c12_34_123_del {Γ₁₂₃₄ Γ₁₂ Γ₃₄ Γ₃ Γ₄ : Ctx? α}
+--   (h12_34 : Γ₁₂₃₄.Split Γ₁₂ Γ₃₄) (h34 : Γ₃₄.Split Γ₃ Γ₄) [h12 : Γ₁₂.del] [h3 : Γ₃.del]
+--   : (h12_34.c12_34_123 h34).del := inferInstance
 
-theorem Ctx?.Split.c12_34_123_copy {Γ₁₂₃₄ Γ₁₂ Γ₃₄ Γ₃ Γ₄ : Ctx? α}
-  (h12_34 : Γ₁₂₃₄.Split Γ₁₂ Γ₃₄) (h34 : Γ₃₄.Split Γ₃ Γ₄) [h12 : Γ₁₂.copy] [h3 : Γ₃.copy]
-  : (h12_34.c12_34_123 h34).copy := inferInstance
+-- theorem Ctx?.Split.c12_34_123_copy {Γ₁₂₃₄ Γ₁₂ Γ₃₄ Γ₃ Γ₄ : Ctx? α}
+--   (h12_34 : Γ₁₂₃₄.Split Γ₁₂ Γ₃₄) (h34 : Γ₃₄.Split Γ₃ Γ₄) [h12 : Γ₁₂.copy] [h3 : Γ₃.copy]
+--   : (h12_34.c12_34_123 h34).copy := inferInstance
 
-abbrev Ctx?.Split.s12_34_123_4 {Γ₁₂₃₄ Γ₁₂ Γ₃₄ Γ₃ Γ₄ : Ctx? α}
-  (h12_34 : Γ₁₂₃₄.Split Γ₁₂ Γ₃₄) (h34 : Γ₃₄.Split Γ₃ Γ₄)
-  : Γ₁₂₃₄.Split (h12_34.c12_34_123 h34) Γ₄ := h12_34.s1_23_12_3 h34
+-- abbrev Ctx?.Split.s12_34_123_4 {Γ₁₂₃₄ Γ₁₂ Γ₃₄ Γ₃ Γ₄ : Ctx? α}
+--   (h12_34 : Γ₁₂₃₄.Split Γ₁₂ Γ₃₄) (h34 : Γ₃₄.Split Γ₃ Γ₄)
+--   : Γ₁₂₃₄.Split (h12_34.c12_34_123 h34) Γ₄ := h12_34.s1_23_12_3 h34
 
-abbrev Ctx?.Split.s12_34_12_3 {Γ₁₂₃₄ Γ₁₂ Γ₃₄ Γ₃ Γ₄ : Ctx? α}
-  (h12_34 : Γ₁₂₃₄.Split Γ₁₂ Γ₃₄) (h34 : Γ₃₄.Split Γ₃ Γ₄)
-  : (h12_34.c12_34_123 h34).Split Γ₁₂ Γ₃ := h12_34.s1_23_12 h34
+-- abbrev Ctx?.Split.s12_34_12_3 {Γ₁₂₃₄ Γ₁₂ Γ₃₄ Γ₃ Γ₄ : Ctx? α}
+--   (h12_34 : Γ₁₂₃₄.Split Γ₁₂ Γ₃₄) (h34 : Γ₃₄.Split Γ₃ Γ₄)
+--   : (h12_34.c12_34_123 h34).Split Γ₁₂ Γ₃ := h12_34.s1_23_12 h34
 
-abbrev Ctx?.Split.c12_34_13 {Γ₁₂₃₄ Γ₁₂ Γ₃₄ Γ₃ Γ₄ : Ctx? α}
-  (h12_34 : Γ₁₂₃₄.Split Γ₁₂ Γ₃₄) (h12 : Γ₁₂.Split Γ₁ Γ₂) (h34 : Γ₃₄.Split Γ₃ Γ₄)
-  : Ctx? α := (h12_34.s12_34_12_3 h34).c12_3_13 h12
+-- abbrev Ctx?.Split.c12_34_13 {Γ₁₂₃₄ Γ₁₂ Γ₃₄ Γ₃ Γ₄ : Ctx? α}
+--   (h12_34 : Γ₁₂₃₄.Split Γ₁₂ Γ₃₄) (h12 : Γ₁₂.Split Γ₁ Γ₂) (h34 : Γ₃₄.Split Γ₃ Γ₄)
+--   : Ctx? α := (h12_34.s12_34_12_3 h34).c12_3_13 h12
 
-theorem Ctx?.Split.c12_34_13_del {Γ₁₂₃₄ Γ₁₂ Γ₃₄ Γ₃ Γ₄ : Ctx? α}
-  (h12_34 : Γ₁₂₃₄.Split Γ₁₂ Γ₃₄) (h12 : Γ₁₂.Split Γ₁ Γ₂) (h34 : Γ₃₄.Split Γ₃ Γ₄)
-  [h1 : Γ₁.del] [h3 : Γ₃.del]
-  : (h12_34.c12_34_13 h12 h34).del := inferInstance
+-- theorem Ctx?.Split.c12_34_13_del {Γ₁₂₃₄ Γ₁₂ Γ₃₄ Γ₃ Γ₄ : Ctx? α}
+--   (h12_34 : Γ₁₂₃₄.Split Γ₁₂ Γ₃₄) (h12 : Γ₁₂.Split Γ₁ Γ₂) (h34 : Γ₃₄.Split Γ₃ Γ₄)
+--   [h1 : Γ₁.del] [h3 : Γ₃.del]
+--   : (h12_34.c12_34_13 h12 h34).del := inferInstance
 
-theorem Ctx?.Split.c12_34_13_copy {Γ₁₂₃₄ Γ₁₂ Γ₃₄ Γ₃ Γ₄ : Ctx? α}
-  (h12_34 : Γ₁₂₃₄.Split Γ₁₂ Γ₃₄) (h12 : Γ₁₂.Split Γ₁ Γ₂) (h34 : Γ₃₄.Split Γ₃ Γ₄)
-  [h1 : Γ₁.copy] [h3 : Γ₃.copy]
-  : (h12_34.c12_34_13 h12 h34).copy := inferInstance
+-- theorem Ctx?.Split.c12_34_13_copy {Γ₁₂₃₄ Γ₁₂ Γ₃₄ Γ₃ Γ₄ : Ctx? α}
+--   (h12_34 : Γ₁₂₃₄.Split Γ₁₂ Γ₃₄) (h12 : Γ₁₂.Split Γ₁ Γ₂) (h34 : Γ₃₄.Split Γ₃ Γ₄)
+--   [h1 : Γ₁.copy] [h3 : Γ₃.copy]
+--   : (h12_34.c12_34_13 h12 h34).copy := inferInstance
 
-abbrev Ctx?.Split.s12_34_13 {Γ₁₂₃₄ Γ₁₂ Γ₃₄ Γ₃ Γ₄ : Ctx? α}
-  (h12_34 : Γ₁₂₃₄.Split Γ₁₂ Γ₃₄) (h12 : Γ₁₂.Split Γ₁ Γ₂) (h34 : Γ₃₄.Split Γ₃ Γ₄)
-  : (h12_34.c12_34_13 h12 h34).Split Γ₁ Γ₃ := (h12_34.s12_34_12_3 h34).s12_3_13 h12
+-- abbrev Ctx?.Split.s12_34_13 {Γ₁₂₃₄ Γ₁₂ Γ₃₄ Γ₃ Γ₄ : Ctx? α}
+--   (h12_34 : Γ₁₂₃₄.Split Γ₁₂ Γ₃₄) (h12 : Γ₁₂.Split Γ₁ Γ₂) (h34 : Γ₃₄.Split Γ₃ Γ₄)
+--   : (h12_34.c12_34_13 h12 h34).Split Γ₁ Γ₃ := (h12_34.s12_34_12_3 h34).s12_3_13 h12
 
-abbrev Ctx?.Split.s12_34_13_2 {Γ₁₂₃₄ Γ₁₂ Γ₃₄ Γ₃ Γ₄ : Ctx? α}
-  (h12_34 : Γ₁₂₃₄.Split Γ₁₂ Γ₃₄) (h12 : Γ₁₂.Split Γ₁ Γ₂) (h34 : Γ₃₄.Split Γ₃ Γ₄)
-  : (h12_34.c12_34_123 h34).Split (h12_34.c12_34_13 h12 h34) Γ₂
-  := (h12_34.s12_34_12_3 h34).s12_3_13_2 h12
+-- abbrev Ctx?.Split.s12_34_13_2 {Γ₁₂₃₄ Γ₁₂ Γ₃₄ Γ₃ Γ₄ : Ctx? α}
+--   (h12_34 : Γ₁₂₃₄.Split Γ₁₂ Γ₃₄) (h12 : Γ₁₂.Split Γ₁ Γ₂) (h34 : Γ₃₄.Split Γ₃ Γ₄)
+--   : (h12_34.c12_34_123 h34).Split (h12_34.c12_34_13 h12 h34) Γ₂
+--   := (h12_34.s12_34_12_3 h34).s12_3_13_2 h12
 
-abbrev Ctx?.Split.c12_34_24 {Γ₁₂₃₄ Γ₁₂ Γ₃₄ Γ₃ Γ₄ : Ctx? α}
-  (h12_34 : Γ₁₂₃₄.Split Γ₁₂ Γ₃₄) (h12 : Γ₁₂.Split Γ₁ Γ₂) (h34 : Γ₃₄.Split Γ₃ Γ₄)
-  : Ctx? α
-  := (h12_34.s12_34_123_4 h34).c12_3_23 (h12_34.s12_34_13_2 h12 h34)
+-- abbrev Ctx?.Split.c12_34_24 {Γ₁₂₃₄ Γ₁₂ Γ₃₄ Γ₃ Γ₄ : Ctx? α}
+--   (h12_34 : Γ₁₂₃₄.Split Γ₁₂ Γ₃₄) (h12 : Γ₁₂.Split Γ₁ Γ₂) (h34 : Γ₃₄.Split Γ₃ Γ₄)
+--   : Ctx? α
+--   := (h12_34.s12_34_123_4 h34).c12_3_23 (h12_34.s12_34_13_2 h12 h34)
 
-theorem Ctx?.Split.c12_34_24_del {Γ₁₂₃₄ Γ₁₂ Γ₃₄ Γ₃ Γ₄ : Ctx? α}
-  (h12_34 : Γ₁₂₃₄.Split Γ₁₂ Γ₃₄) (h12 : Γ₁₂.Split Γ₁ Γ₂) (h34 : Γ₃₄.Split Γ₃ Γ₄)
-  [h2 : Γ₂.del] [h4 : Γ₄.del]
-  : (h12_34.c12_34_24 h12 h34).del := inferInstance
+-- theorem Ctx?.Split.c12_34_24_del {Γ₁₂₃₄ Γ₁₂ Γ₃₄ Γ₃ Γ₄ : Ctx? α}
+--   (h12_34 : Γ₁₂₃₄.Split Γ₁₂ Γ₃₄) (h12 : Γ₁₂.Split Γ₁ Γ₂) (h34 : Γ₃₄.Split Γ₃ Γ₄)
+--   [h2 : Γ₂.del] [h4 : Γ₄.del]
+--   : (h12_34.c12_34_24 h12 h34).del := inferInstance
 
-theorem Ctx?.Split.c12_34_24_copy {Γ₁₂₃₄ Γ₁₂ Γ₃₄ Γ₃ Γ₄ : Ctx? α}
-  (h12_34 : Γ₁₂₃₄.Split Γ₁₂ Γ₃₄) (h12 : Γ₁₂.Split Γ₁ Γ₂) (h34 : Γ₃₄.Split Γ₃ Γ₄)
-  [h2 : Γ₂.copy] [h4 : Γ₄.copy]
-  : (h12_34.c12_34_24 h12 h34).copy := inferInstance
+-- theorem Ctx?.Split.c12_34_24_copy {Γ₁₂₃₄ Γ₁₂ Γ₃₄ Γ₃ Γ₄ : Ctx? α}
+--   (h12_34 : Γ₁₂₃₄.Split Γ₁₂ Γ₃₄) (h12 : Γ₁₂.Split Γ₁ Γ₂) (h34 : Γ₃₄.Split Γ₃ Γ₄)
+--   [h2 : Γ₂.copy] [h4 : Γ₄.copy]
+--   : (h12_34.c12_34_24 h12 h34).copy := inferInstance
 
-abbrev Ctx?.Split.s12_34_13_24 {Γ₁₂₃₄ Γ₁₂ Γ₃₄ Γ₃ Γ₄ : Ctx? α}
-  (h12_34 : Γ₁₂₃₄.Split Γ₁₂ Γ₃₄) (h12 : Γ₁₂.Split Γ₁ Γ₂) (h34 : Γ₃₄.Split Γ₃ Γ₄)
-  : Γ₁₂₃₄.Split (h12_34.c12_34_13 h12 h34) (h12_34.c12_34_24 h12 h34)
-  := (h12_34.s12_34_123_4 h34).s12_3_1_23 (h12_34.s12_34_13_2 h12 h34)
+-- abbrev Ctx?.Split.s12_34_13_24 {Γ₁₂₃₄ Γ₁₂ Γ₃₄ Γ₃ Γ₄ : Ctx? α}
+--   (h12_34 : Γ₁₂₃₄.Split Γ₁₂ Γ₃₄) (h12 : Γ₁₂.Split Γ₁ Γ₂) (h34 : Γ₃₄.Split Γ₃ Γ₄)
+--   : Γ₁₂₃₄.Split (h12_34.c12_34_13 h12 h34) (h12_34.c12_34_24 h12 h34)
+--   := (h12_34.s12_34_123_4 h34).s12_3_1_23 (h12_34.s12_34_13_2 h12 h34)
 
-abbrev Ctx?.Split.s12_34_24 {Γ₁₂₃₄ Γ₁₂ Γ₃₄ Γ₃ Γ₄ : Ctx? α}
-  (h12_34 : Γ₁₂₃₄.Split Γ₁₂ Γ₃₄) (h12 : Γ₁₂.Split Γ₁ Γ₂) (h34 : Γ₃₄.Split Γ₃ Γ₄)
-  : (h12_34.c12_34_24 h12 h34).Split Γ₂ Γ₄
-  := (h12_34.s12_34_123_4 h34).s12_3_23 (h12_34.s12_34_13_2 h12 h34)
+-- abbrev Ctx?.Split.s12_34_24 {Γ₁₂₃₄ Γ₁₂ Γ₃₄ Γ₃ Γ₄ : Ctx? α}
+--   (h12_34 : Γ₁₂₃₄.Split Γ₁₂ Γ₃₄) (h12 : Γ₁₂.Split Γ₁ Γ₂) (h34 : Γ₃₄.Split Γ₃ Γ₄)
+--   : (h12_34.c12_34_24 h12 h34).Split Γ₂ Γ₄
+--   := (h12_34.s12_34_123_4 h34).s12_3_23 (h12_34.s12_34_13_2 h12 h34)
